Finset proofs wrt `castSucc` and `castPred` ⬆⬇
- Introduce `OF-0`, `OF-1`
- `castSucc`, `castPred` for `Finset`
- Leave some interesting open ideas as TODOs

RuleSystem/Rules/Finset.lean
@@ -1,3 +1,4 @@
+import Mathlib.Data.Fintype.Basic
 import Mathlib.Data.Finset.Image
 import RuleSystem.Rules.Fin
 
@@ -8,29 +9,65 @@ namespace Finset
 instance instCoeOutSubtype {α : Type*} {p : α → Prop} : CoeOut (Finset (Subtype p)) (Finset α) where
   coe := map (Function.Embedding.subtype _)
 
-theorem castPred_mem_iff_mem_map_castSuccEmb
+def castSucc {n : ℕ} (s : Finset (Fin n)) : Finset (Fin (n + 1)) := s.map Fin.castSuccEmb
+
+def castSuccEmbedding {n : ℕ} : Finset (Fin n) ↪ Finset (Fin (n + 1))
+  := ⟨castSucc, by simp [Function.Injective, castSucc]⟩
+
+def CastPredPrecondition {n : ℕ} (s : Finset (Fin (n + 1))) := ∀ x ∈ s, x ≠ Fin.last _
+
+-- Restrict `Fin.castPred` to members of `s` given `s.CastPredPrecondition`.
+def restrictFinCastPred {n : ℕ} (s : Finset (Fin (n + 1))) (h : s.CastPredPrecondition) (x : s) : Fin n :=
+  -- TODO: Why does this work but not the commented out version below?
+  x.restrict (· ∈ s) Fin.castPred (h x x.property)
+  -- Subtype.restrict (· ∈ s) (λ (y : s) ↦ Fin.castPred y (h y y.property)) x
+
+def restrictFinCastPred_injective {n : ℕ} (s : Finset (Fin (n + 1))) (h : s.CastPredPrecondition)
+  : Function.Injective (restrictFinCastPred s h) := by
+    intro x y castPred_x_eq_castPred_y
+    simp [restrictFinCastPred] at castPred_x_eq_castPred_y
+    apply Subtype.eq
+    exact Fin.castPred_inj.mp castPred_x_eq_castPred_y
+
+def castPred {n : ℕ} (s : Finset (Fin (n + 1))) (h : s.CastPredPrecondition) : Finset (Fin n) :=
+  -- TODO: Why does this work but not the commented out version below?
+  Finset.univ.map ⟨restrictFinCastPred s h, restrictFinCastPred_injective s h⟩
+  -- s.map ⟨restrictFinCastPred s h, restrictFinCastPred_injective s h⟩
+
+-- TODO: Do we want to use this definition? It's certainly nicer to write down
+def castPred' {n : ℕ} (s : Subtype (@CastPredPrecondition n)) := castPred s.val s.property
+
+theorem castPred_mem_iff_mem_castSucc
     {n : ℕ}
     {x : Fin (n + 1)}
     {x_ne_last : x ≠ Fin.last _}
     {s : Finset (Fin n)}
-  : x.castPred x_ne_last ∈ s ↔ x ∈ s.map Fin.castSuccEmb := by
-    simp [Fin.castLE] at *
+  : x.castPred x_ne_last ∈ s ↔ x ∈ s.castSucc := by
+    simp [castSucc, Fin.castLE] at *
     constructor
     · intro
       exists x.castPred x_ne_last
-    · intro x_mem_map_castSuccEmb
-      obtain ⟨_, _, _⟩ := x_mem_map_castSuccEmb
+    · intro x_mem_map_castSucc
+      obtain ⟨_, _, _⟩ := x_mem_map_castSucc
       subst x
       assumption
 
--- TODO: There should be a more general version of this, find and prove it
+-- TODO: Finish this 🟠
+theorem castSucc_mem_iff_mem_castPred
+    {n : ℕ}
+    {x : Fin n}
+    {s : Finset (Fin (n + 1))}
+    (s_castPredPrecondition : s.CastPredPrecondition)
+  : x.castSucc ∈ s ↔ x ∈ s.castPred s_castPredPrecondition := by
+    sorry
+
+-- TODO: There should be an even more general version of this, find and prove it. Can we just use any embedding?
 -- TODO: Naming
--- tags_inter_inst'_tags_eq_empty : tags ∩ inst'.tags = ∅
--- ⊢ Finset.map Fin.castSuccEmb tags ∩ Finset.map Fin.castSuccEmb inst'.tags = ∅
-theorem inter_eq_empty_iff_inter_map_castSuccEmb_eq_empty
+-- 🔮 (OF-0): `· · ↑ ↑`
+theorem inter_eq_empty_iff_castSucc_inter_castSucc_eq_empty
     {n : ℕ}
     {s t : Finset (Fin n)}
-  : s ∩ t = ∅ ↔ s.map Fin.castSuccEmb ∩ t.map Fin.castSuccEmb = ∅ := by
+  : s ∩ t = ∅ ↔ s.castSucc ∩ t.castSucc = ∅ := by
     constructor
     -- TODO: Maybe there's an easier way, this is all very technical
     · intro inter_eq_empty
@@ -41,16 +78,16 @@ theorem inter_eq_empty_iff_inter_map_castSuccEmb_eq_empty
           obtain ⟨x, x_mem_inter_map_castSuccEmb⟩ := Finset.nonempty_of_ne_empty inter_map_castSuccEmb_ne_empty
           have x_ne_last : x ≠ Fin.last n := by
             intro x_eq_last
-            simp [x_eq_last, Fin.castSuccEmb] at x_mem_inter_map_castSuccEmb
+            simp [x_eq_last, castSucc, Fin.castSuccEmb] at x_mem_inter_map_castSuccEmb
             obtain ⟨⟨_, _, castLE_eq_last⟩, _⟩ := x_mem_inter_map_castSuccEmb
             exact Fin.false_of_castLE_eq_last castLE_eq_last
           set x' := x.castPred x_ne_last with x'_def
           have x'_mem_inter : x' ∈ s ∩ t := by
             simp [x'_def]
             constructor
-            · apply castPred_mem_iff_mem_map_castSuccEmb.mpr
+            · apply castPred_mem_iff_mem_castSucc.mpr
               exact (Finset.mem_inter.mp x_mem_inter_map_castSuccEmb).left
-            · apply castPred_mem_iff_mem_map_castSuccEmb.mpr
+            · apply castPred_mem_iff_mem_castSucc.mpr
               exact (Finset.mem_inter.mp x_mem_inter_map_castSuccEmb).right
           simp [inter_eq_empty] at x'_mem_inter
         | inr r_ne_empty =>
@@ -74,12 +111,56 @@ theorem inter_eq_empty_iff_inter_map_castSuccEmb_eq_empty
       by_contra inter_ne_empty
       obtain ⟨x, x_mem_inter⟩ := Finset.nonempty_of_ne_empty inter_ne_empty
       set x' := x.castSucc with x'_def
-      have x'_mem_map_castSuccEmb : x' ∈ (s.map Fin.castSuccEmb ∩ t.map Fin.castSuccEmb) := by
+      have x'_mem_inter_castSucc : x' ∈ (s.castSucc ∩ t.castSucc) := by
         apply Finset.mem_inter_of_mem
-        · simp [x'_def, Fin.castSucc, Fin.castAdd]
+        · simp [castSucc, x'_def, Fin.castSucc, Fin.castAdd]
           exact Finset.mem_of_mem_inter_left x_mem_inter
-        · simp [x'_def, Fin.castSucc, Fin.castAdd]
+        · simp [castSucc, x'_def, Fin.castSucc, Fin.castAdd]
           exact Finset.mem_of_mem_inter_right x_mem_inter
-      simp [inter_map_castSuccEmb_eq_empty] at x'_mem_map_castSuccEmb
+      simp [inter_map_castSuccEmb_eq_empty] at x'_mem_inter_castSucc
+
+-- TODO: There should be an even more general version of this, find and prove it. Can we just use any embedding and it's
+--       "inverse" in the sense that `castPred` is an inverse here
+-- TODO: Naming
+-- TODO: Formulate with `castPred'`
+-- 🔮 (OF-1): `· ↓ ↑ ·`
+theorem inter_castPred_eq_empty_iff_castSucc_inter_eq_empty
+    {n : ℕ}
+    {s : Finset (Fin n)}
+    {t : Finset (Fin (n + 1))}
+    (t_castPredPrecondition : t.CastPredPrecondition)
+  : s ∩ (t.castPred t_castPredPrecondition) = ∅ ↔ s.castSucc ∩ t = ∅ := by
+    -- TODO: Very similar to above, maybe we can factor out common stuff
+    constructor
+    · intro inter_castPred_eq_empty
+      by_contra castSucc_inter_ne_empty
+      obtain ⟨x, x_mem_castSucc_inter⟩ := Finset.nonempty_of_ne_empty castSucc_inter_ne_empty
+      have x_ne_last : x ≠ Fin.last _ := by
+        intro x_eq_last
+        simp [x_eq_last, castSucc] at x_mem_castSucc_inter
+        obtain ⟨⟨_, _, castLE_eq_last⟩, _⟩ := x_mem_castSucc_inter
+        exact Fin.false_of_castLE_eq_last castLE_eq_last
+      set x' := x.castPred x_ne_last with x'_def
+      have x'_mem_inter_castPred : x' ∈ s ∩ (t.castPred t_castPredPrecondition) := by
+        simp [x'_def]
+        constructor
+        · apply castPred_mem_iff_mem_castSucc.mpr
+          exact (Finset.mem_inter.mp x_mem_castSucc_inter).left
+        · simp [castPred, restrictFinCastPred, Subtype.restrict]
+          exists x
+          exists (Finset.mem_inter.mp x_mem_castSucc_inter).right
+      simp [inter_castPred_eq_empty] at x'_mem_inter_castPred
+    · intro castSucc_inter_eq_empty
+      by_contra inter_castPred_ne_empty
+      obtain ⟨x, x_mem_inter_castPred⟩ := Finset.nonempty_of_ne_empty inter_castPred_ne_empty
+      set x' := x.castSucc with x'_def
+      have x'_mem_castSucc_inter : x' ∈ (s.castSucc ∩ t) := by
+        apply Finset.mem_inter_of_mem
+        · simp [castSucc, x'_def, Fin.castSucc, Fin.castAdd]
+          exact Finset.mem_of_mem_inter_left x_mem_inter_castPred
+        · simp [x'_def]
+          apply (castSucc_mem_iff_mem_castPred t_castPredPrecondition).mpr
+          exact Finset.mem_of_mem_inter_right x_mem_inter_castPred
+      simp [castSucc_inter_eq_empty] at x'_mem_castSucc_inter
 
 end Finset
