RuleSystem.lean
@@ -1,3 +1,8 @@
 -- This module serves as the root of the `RuleSystem` library.
 -- Import modules here that should be built as part of the library.
-import RuleSystem.Basic
+import RuleSystem.Rules.Theorems.Basic
+import RuleSystem.Rules.Theorems.Advanced
+import RuleSystem.Rules.Theorems.Wip
+import RuleSystem.Rules.Theorems.Embeddings.All
+import RuleSystem.Rules.Theorems.Embeddings.Positive
+import RuleSystem.Rules.Theorems.Embeddings.Negative
